finished the Monad instance for StateT

theories/MonadState.v
@@ -61,204 +61,23 @@ Global Instance StateT_MonadOps : MonadOps StateT :=
        fun s => do s_x <- m s; f (snd s_x) (fst s_x);
    lrM := fun {A} _ => LR_Op_fun }.
 
-
 (* The Monad instance for StateT *)
 Global Instance StateT_Monad : Monad (StateT).
 Proof.
-  constructor; intros; unfold returnM, bindM, lrM, StateT_MonadOps;
-  try apply LR_fun; try prove_lr; try prove_lr_proper.
-  admit. (* FIXME HERE NOW *)
-  transitivity (do s_x <- m x; returnM s_x); prove_lr.
-
-  FIXME HERE NOW: the above could maybe be done with an alternative monad-return-bind...?
-
-  Print apply_lr_leq.
-
-  match goal with
-  | |- (?f _) <~ (?g _) => apply apply_lr_leq; [ change (f <~ g) | ]; prove_lr
-  end.
-
-  rewrite Rxy.
-
-  prove_lr_proper.
-  prove_lr_proper.
-  admit.
-  autorewrite with LR.
-
-  build_lr_fun; prove_lr.
-  
-  lazymatch goal with
-  | |- _ <~ (fun _ => _) =>
-    let x := fresh "x" in
-    let y := fresh "y" in
-    let Rxy := fresh "Rxy" in
-    apply Build_LRFun; intros x y Rxy; prove_lr
-  end.
-  
-  split; intros foo1 foo2 Rfoo; prove_lr.
-
-  { apply LR_fun. }
-  {
-  repeat (first [ solve [ eauto with typeclass_instances ]
-                | progress (apply fun_Proper_lr_leq)
-                | apply fun_Proper_lr_leq_adjoint
-                | apply fun_Proper_arrow_pair_commute
-                | apply fun_Proper_arrow_adjoint ]).
-  repeat (intro; intros).
-  apply apply_lr_leq; [ change (returnM <~ (returnM : S * A -> M (S * A))) | ].
-  lazymatch goal with
-  | |- ?f <~ ?g =>
-    first [ change (Proper lr_leq f) (* ; solve [ eauto with typeclass_instances ] *)
-          | change (f <~ f); assumption_semi_refl
-          | assumption
-          | idtac ]
-  end.
-  Print HintDb typeclass_instances.
-  auto with typeclass_instances.
-  apply monad_proper_return.
-
-
-  prove_lr.
-    first [ change (Proper lr_leq f); solve [ eauto with typeclass_instances ]
-          | change (returnM <~ (returnM : S * A -> M (S * A))); assumption_semi_refl
-          | assumption
-          | idtac ].
-
-
- prove_lr.
-
- prove_lr_proper.
-
-  { apply LR_fun. }
-  { intros x y Rxy. intros s1 s2 Rs.
-    repeat split; apply monad_proper_return; split.
-      try assumption.
-      [ apply (semi_reflexivity _ y); left
-      | apply (semi_reflexivity _ x); right ]; assumption. }
-  { intros m1 m2 Rm f1 f2 Rf s1 s2 Rs; repeat split;
-      apply (monad_proper_bind (M:=M)); try ( apply Rm; assumption );
-        intros p1 p2 Rp; repeat split; apply Rf; apply Rp. }
-  { intros R1 R2 sub m1 m2 Rm s1 s2 Rs. repeat split;
-      ( eapply monad_proper_lrM;
-        [ intros p1 p2 Rp; split; try apply sub
-        | apply Rm; assumption ]); apply Rp. }
-  { unfold returnM, bindM, StateT_MonadOps.
-
-    split; intros s1 s2 sub_s; repeat split. try apply (monad_proper_bind (M:=M)).
+  constructor; intros; unfold StateT, returnM, bindM, lrM, StateT_MonadOps.
+  - auto with typeclass_instances.
+  - prove_lr_proper.
+  - prove_lr_proper.
+  - intros R1 R2 subR; apply LRFun_Proper_subrelation; apply monad_proper_lrM;
+      apply LRPair_Proper_subrelation; try assumption; reflexivity.
+  - prove_lr.
+  - transitivity (fun s => do s_x <- m s; returnM s_x).
+    + split; build_lr_fun; apply monad_proper_bind; prove_lr.
+    + prove_lr.
+  - prove_lr.
+Qed.
 
 FIXME HERE NOW
-
-  { eapply StateT_Equals. }
-  { red. red. intros.
-    eapply monad_proper_return; tc.
-    split. reflexivity. assumption. }
-  { do 4 red. intros.
-    eapply monad_proper_bind; tc.
-    red. intros.
-    destruct x1; destruct y1. destruct H4; simpl in *.
-    subst. eapply H3. assumption. }
-  { red. red. unfold subrelation.
-    intros.
-    eapply monad_proper_equalsM. 2: eapply H1.
-    red. intros; auto. unfold S_EqualsOp in *.
-    destruct H2; split; auto.
-    unfold equals in *. eapply H0. assumption. }
-Qed.
-
-
-
-
-Record StateResult (T : Type) : Type := mkStResult
-{ state : S ; result : T }.
-
-Arguments mkStResult {_} _ _.
-Arguments state {_} _.
-Arguments result {_} _.
-
-(* NOTE: StateT requires that propositional equality, eq, be used as the
-distinguished equality for the state type, S. Otherwise, we need to restrict
-StateT to only contain Proper functions from S, which seems like a pain. *)
-Global Instance S_EqualsOp {A} `{EqualsOp A} : EqualsOp (StateResult A) :=
-  fun a b => a.(state) = b.(state) /\ equals a.(result) b.(result).
-Global Instance S_Equals {A} `{Equals A} : Equals (StateResult A).
-Proof.
-  constructor. constructor.
-  - constructor; auto. eapply reflexivity.
-  - red. destruct 1. constructor; auto. symmetry. auto.
-  - red. destruct 1. destruct 1. constructor. congruence. rewrite H1. assumption.
-Qed.
-
-(* StateT itself *)
-Variable M : Type -> Type.
-
-Definition StateT (X:Type) := S -> M (StateResult X).
-
-Global Instance StateT_EqualsOp {A} `{MonadOps M} `{EqualsOp A} : EqualsOp (StateT A) :=
-  pointwise_relation S equals.
-Global Instance StateT_Equals {A} `{Monad M} `{Equals A} : Equals (StateT A).
-Proof.
-  constructor; constructor.
-  { red. intro. reflexivity. }
-  { red. intro. symmetry. assumption. }
-  { red. intro. etransitivity; eauto. }
-Qed.
-
-Global Instance StateT_MonadOps `{MonadOps M} : MonadOps StateT :=
-  {returnM :=
-     fun A x => fun s => returnM (mkStResult s x);
-   bindM :=
-     fun A B m f =>
-       fun s => bindM (m s) (fun sx => let '(mkStResult s' x) := sx in f x s');
-   equalsM :=
-     fun {A} {EqualsOp} m1 m2 =>
-       forall s, (m1 s) == (m2 s) }.
-
-Ltac tc := eauto with typeclass_instances.
-
-(* The Monad instance for StateT *)
-Global Instance StateT_Monad `{Monad M} : Monad (StateT).
-  constructor; simpl; intros.
-  { red. intros.
-    rewrite (monad_return_bind (M:=M));
-      try auto with typeclass_instances; reflexivity. }
-  { red; intros.
-    etransitivity.
-    eapply (monad_proper_bind (M:=M)). tc. tc. reflexivity.
-    instantiate (1 := returnM).
-    red. intros. destruct x. eapply monad_proper_return; tc.
-    eapply (monad_bind_return (M:=M)). tc. }
-  { red. intros.
-    rewrite monad_assoc; tc.
-    eapply bind_fun_equalsM. intros.
-    destruct x. reflexivity. }
-  { eapply StateT_Equals. }
-  { red. red. intros.
-    eapply monad_proper_return; tc.
-    split. reflexivity. assumption. }
-  { do 4 red. intros.
-    eapply monad_proper_bind; tc.
-    red. intros.
-    destruct x1; destruct y1. destruct H4; simpl in *.
-    subst. eapply H3. assumption. }
-  { red. red. unfold subrelation.
-    intros.
-    eapply monad_proper_equalsM. 2: eapply H1.
-    red. intros; auto. unfold S_EqualsOp in *.
-    destruct H2; split; auto.
-    unfold equals in *. eapply H0. assumption. }
-Qed.
-
-Global Instance StateT_getM `{Monad M} : MonadStateOps S (StateT) :=
-{ getM := fun s => returnM (mkStResult s s)
-; putM := fun s_new s => returnM (mkStResult s_new tt) }.
-
-Definition EqualsOp_Libniz (T : Type) : EqualsOp T := @eq T.
-Definition Equals_Libniz (T : Type) : @Equals T (EqualsOp_Libniz T).
-Proof.
-  constructor. compute. tc.
-Qed.
-
-Local Existing Instance Equals_Libniz.
 
 Instance StateT_MonadState `{Monad M}
 : @MonadState S StateT (EqualsOp_Libniz S) _ _.
